\documentclass{article}
\usepackage{amsmath}

\title{Math Proofs}
\author{Andrew Archibald}
\date{July 2017}

\begin{document}

\begin{titlepage}
\maketitle
\end{titlepage}

\section{Pi by the sum of inverse squares}

$$\frac{\pi^2}{6} = \sum_{n=1}^{\infty}\frac{1}{n^2}$$

\section{Pi by inverse tangent Taylor series}

\begin{align*}
\arctan x &= x - \frac{x^3}{3} + \frac{x^5}{5} - \frac{x^7}{7} + \frac{x^9}{9} - \cdots \\
          &= \sum_{n=0}^{\infty} (-1)^n \frac{x^{2n + 1}}{2n + 1}
\end{align*}
$$x \in [-1, 1]$$
$$\frac{\pi}{4} = \arctan 1
= \sum_{n=0}^{\infty} \frac{(-1)^n}{2n + 1}$$

\section{Pi by inscribed and circumscribed polygons}

\subsection{Inscribed}

\subsubsection{Law of sines}

$$\frac{\sin(\frac{\pi}{2}-\frac{\pi}{n})}{r} = \frac{\sin\frac{2\pi}{n}}{l}$$
$$= \frac{\cos\frac{\pi}{n}}{r} = \frac{2\sin\frac{\pi}{n}\cos\frac{\pi}{n}}{l}$$
$$l = 2r\sin\frac{\pi}{n}$$
$$P = ln
= 2rn\sin\frac{\pi}{n}$$

\subsubsection{Law of cosines}

$$l^2 = 2r^2 - 2r^2cos\frac{2\pi}{n}
= 2r^2\left(1 - cos\frac{2\pi}{n}\right)
= 4r^2\left(\frac{1 - cos\frac{2\pi}{n}}{2}\right)
= 4r^2\sin^2{\frac{\pi}{n}}$$
$$l = 2r\sin\frac{\pi}{n} = r\sqrt{2 - 2\cos\frac{2\pi}{n}}$$
$$P = 2n\sin\frac{\pi}{n}$$

\subsubsection{Pythagorean theorem}

$$r^2 = \left(\frac{l}{2}\right)^2 + h^2$$
$$h^2 = r^2 - \frac{1}{4}l^2
= r^2 - r^2\sin^2\frac{\pi}{n}
= r^2\left(1 - \sin^2\frac{\pi}{n}\right)
= r^2\cos^2\frac{\pi}{n}$$
$$h = r\cos\frac{\pi}{n}$$
$$A = \frac{1}{2}lhn
= \frac{1}{2}\left(2r\sin\frac{\pi}{n}\right)\left(rcos\frac{\pi}{n}\right)n
= nr^2\sin\frac{\pi}{n}\cos\frac{\pi}{n}
= \frac{1}{2}nr^2\sin\frac{2\pi}{n}$$

\subsubsection{Results}

Perimeter

$$2\pi{r} = \lim_{n\to\infty} P
= \lim_{n\to\infty} 2rn\sin\frac{\pi}{n}$$

Area

$$\pi{r^2} = \lim_{n\to\infty} \frac{1}{2}nr^2\sin\frac{2\pi}{n}$$
$$\pi = \lim_{n\to\infty} \frac{1}{2}n\sin\frac{2\pi}{n}
= \lim_{n\to\infty} n\sin\frac{\pi}{n}\cos\frac{\pi}{n}$$

\subsection{Circumscribed}

\subsubsection{Law of sines}

$$\frac{\sin\frac{\pi}{n}}{L} = \frac{\sin\left(\pi - \frac{2\pi}{n}\right)}{l}$$
$$\sin\left(\pi - \frac{2\pi}{n}\right) = \sin\left[2\left(\frac{\pi}{2} - \frac{\pi}{n}\right)\right]
= 2\sin\left(\frac{\pi}{2} - \frac{\pi}{n}\right)\cos\left(\frac{\pi}{2} - \frac{\pi}{n}\right)
= 2\sin\frac{\pi}{n}\cos\frac{\pi}{n}$$
$$L = \frac{l\sin\frac{\pi}{n}}{2\sin\frac{\pi}{n}\cos\frac{\pi}{n}}
= \frac{1}{2}l\sec\frac{\pi}{n}
= \frac{1}{2}\left(2r\sin\frac{\pi}{n}\right)\sec\frac{\pi}{n}
= r\tan\frac{\pi}{n}$$

\subsubsection{Law of cosines}

$$l^2 = 2L^2 - 2L^2cos\frac{\pi - 2\pi}{n}
= L^2\left(2 - 2\cos\left(\pi - \frac{2\pi}{n}\right)\right)$$
$$\cos\left(\pi - \frac{2\pi}{n}\right) = \cos\left(2\left(\frac{\pi}{2} - \frac{\pi}{n}\right)\right)
= 1 - 2\sin^2\left(\frac{\pi}{2} - \frac{\pi}{n}\right)
= 1 - 2\cos^2\frac{\pi}{2}$$
$$l^2 = L^2\left[2 - 2\left(1 - 2\cos^2\frac{\pi}{n}\right)\right]
= 4L^2\cos^2\frac{\pi}{n}$$
$$l = 2L\cos\frac{\pi}{n}$$
$$2r\sin\frac{\pi}{n} = 2L\cos{\pi}{n}$$
$$L = r\tan\frac{\pi}{n}$$

\subsubsection{Pythagorean theorem}

$$L^2 = \left(\frac{l}{2}\right)^2 + H^2$$
$$H^2 = r^2tan^2\frac{\pi}{n} - r^2\sin^2\frac{\pi}{n}
= r^2\left(\tan^2\frac{\pi}{n} - \sin^2\frac{\pi}{n}\right)$$
$$tan^2\frac{\pi}{n} - \sin^2\frac{\pi}{n} = tan^2\frac{\pi}{n} - \cos^2\frac{\pi}{2}\tan\frac{\pi}{2}
= \tan^2\frac{\pi}{n}\left(1 - \cos^2\frac{\pi}{n}\right)
= \sin^2\frac{\pi}{n}tan^2\frac{\pi}{n}$$
$$H^2 = R^2sin^2\frac{\pi}{n}\tan^2{\pi}{n}$$
$$H = r\sin\frac{\pi}{n}\tan\frac{\pi}{n}$$

\subsubsection{Results}

Perimeter

$$P = 2nL = 2nr\tan\frac{\pi}{n}$$
$$2\pi{r} = \lim_{n\to\infty} 2nr\tan\frac{\pi}{n}$$
$$\pi = \lim_{n\to\infty} n\tan\frac{\pi}{n}$$

Area

$$A = nH\frac{L}{2} + A_l$$
$$  = n\left(r\sin\frac{\pi}{n}\tan\frac{\pi}{n}\right)\left(r\sin\frac{\pi}{n}\right) + A_l$$
$$  = nr^2\sin^2\frac{\pi}{n}\tan\frac{\pi}{n} + A_l$$
$$  = nr^2\sin^2\frac{\pi}{n}\tan\frac{\pi}{n} + nr^2\sin\frac{\pi}{n}\cos\frac{\pi}{n}$$
$$  = nr^2\sin\frac{\pi}{n}\left(\sin\frac{\pi}{n}\tan\frac{\pi}{n} + \cos\frac{\pi}{n}\right)$$
$$  = nr^2\tan\frac{\pi}{n}\left(\sin^2\frac{\pi}{n} + \cos^2\frac{\pi}{n}\right)$$
$$  = nr^2\tan\frac{\pi}{n}$$
$$\pi{r^2} = \lim_{n\to\infty} nr^2\tan\frac{\pi}{n}$$
$$\pi = \lim_{n\to\infty} n\tan\frac{\pi}{n}$$

\subsection{Simplified results}

$$\pi = \lim_{n\to\infty} n\sin\frac{\pi}{n}$$
$$\pi = \lim_{n\to\infty} n\sin\frac{\pi}{n}\cos\frac{\pi}{n}$$
$$\pi = \lim_{n\to\infty} n\tan\frac{\pi}{n}$$

\section{Multi-dimensional spheres}

$$V_1 = \int\limits_{-R}^{R} dx = 2R$$
$$V_2
= \int\limits_{-R}^{R} \int_{-\sqrt{R^2-x^2}}^{\sqrt{R^2-x^2}} dydx
= \int\limits_{-R}^{R} 2\sqrt{R^2-x^2} dx
= \int\limits_{-R}^{R} 2R\sin\arccos\frac{x}{R} dx$$
$$V_2
= \int\limits_0^{2\pi} \int\limits_0^{R} r drd\theta
= \int\limits_0^{2\pi} \frac{1}{2}R^2 d\theta
= \pi R^2$$

\section{Trigonometric integrals}

\begin{align*}
\int \sin^2{x} dx
  &= \int \frac{1-\cos{2x}}{2} dx \\
  &= \frac{1}{2}(x - \sin{x}\cos{x}) + C
\\\\
\int \cos^2{x} dx
  &= \int \frac{1+\cos{2x}}{2} dx \\
  &= \frac{1}{2}(x + \sin{x}\cos{x}) + C
\end{align*}

\begin{align*}
\int \sin^3{x} dx
  &= \int (1-\cos^2{x})\sin{x} dx \\
  &= \int (\sin{x} - \cos^2{x}\sin{x}) dx \\
  &= -\cos{x} + \frac{1}{3}\cos^3{x} + C
\\\\
\int \cos^3{x} dx
  &= \int (1-\sin^2{x})\cos{x} dx \\
  &= \int (\cos{x} - \sin^2{x}\cos{x}) dx \\
  &= \sin{x} - \frac{1}{3}\sin^3{x} + C
\end{align*}

\begin{align*}
\int \sin^4{x} dx
  &= \int \left(\frac{1 -\cos{2x}}{2}\right)^2 dx \\
  &= \int \frac{1}{4}(1 - 2\cos{2x} + \cos^2{2x}) dx \\
  &= \int \frac{1}{4}(1 - 2\cos{2x} + \frac{1 + \cos{4x}}{2}) dx \\
  &= \int \frac{1}{8}(3 - 4\cos{2x} + \cos{4x}) dx \\
  &= \frac{1}{8}(3x - 2\sin{2x} + \frac{1}{4}\sin{4x}) + C
\\\\
\int \cos^4{x} dx
  &= \int \left(\frac{1 +\cos{2x}}{2}\right)^2 dx \\
  &= \int \frac{1}{4}(1 + 2\cos{2x} + \cos^2{2x}) dx \\
  &= \int \frac{1}{4}(1 + 2\cos{2x} + \frac{1 + \cos{4x}}{2}) dx \\
  &= \int \frac{1}{8}(3 + 4\cos{2x} + \cos{4x}) dx \\
  &= \frac{1}{8}(3x + 2\sin{2x} + \frac{1}{4}\sin{4x}) + C
\end{align*}

\begin{align*}
\int \sin^5{x} dx
  &= \int (1 - \cos^2{x})^2\sin{x} dx \\
  &= \int (\sin{x} - 2\cos^2{x}\sin{x} + \cos^4{x}\sin{x}) dx \\
  &= -\cos{x} + \frac{2}{3}\cos^3{x} - \frac{1}{5}\cos^5{x} + C
\\\\
\int \cos^5{x} dx
  &= \int (1 - \sin^2{x})^2\cos{x} dx \\
  &= \int (\cos{x} - 2\sin^2{x}\cos{x} + \sin^4{x}\cos{x}) dx \\
  &= \sin{x} - \frac{2}{3}\sin^3{x} + \frac{1}{5}\sin^5{x} + C
\end{align*}

\end{document}
